backend/Asmgenproof0.v
@@ -949,10 +949,9 @@ Proof.
       now rewrite Pos.eqb_refl.
     - eapply exec_step_internal_return; eauto.
       eapply find_instr_tail. eauto.
-      now rewrite H0, H2.
-      simpl; now rewrite H3.
-      simpl; now rewrite H3.
-      right; left; simpl. now rewrite H3.
+      now rewrite H0, H2; simpl; rewrite H3.
+      now rewrite H0, H2; simpl; rewrite H3.
+      congruence. congruence.
       unfold update_stack_return.
       rewrite H0, H2; simpl; rewrite H3.
       now rewrite Pos.eqb_refl.
@@ -976,10 +975,9 @@ Proof.
       now rewrite Pos.eqb_refl.
     - eapply exec_step_internal_return; eauto.
       eapply find_instr_tail. eauto.
-      now rewrite H0, H3.
-      simpl; now rewrite H4.
-      simpl; now rewrite H4.
-      right; left; simpl. now rewrite H4.
+      now rewrite H0, H3; simpl; rewrite H4.
+      now rewrite H0, H3; simpl; rewrite H4.
+      congruence. congruence.
       unfold update_stack_return.
       rewrite H0, H3; simpl; rewrite H4.
       now rewrite Pos.eqb_refl.
